Blum's iterated zero-knowledge

case_studies/HamiltonBlum/Blum_Sim1Property.ec
@@ -28,39 +28,53 @@ module ZKP(P : HonestProver, V : MaliciousVerifier) = {
 }.
 
 
+
+module ZKP' = {
+  proc run(Ny : hc_prob, w : hc_wit, b : bool) = {
+    var c,r,prm,fal,pi_gwco,pi_w;
+
+    prm <$ perm_d K;
+    fal <- permute_graph prm Ny;
+    pi_gwco <$ djoinmap Com fal;
+    c <- (unzip1 pi_gwco);
+
+    pi_w <- permute_witness prm w;
+    r <- if b then Left (prm, unzip2 pi_gwco) else Right (pi_w, unzip2 (prj_path pi_w pi_gwco));
+    return (c, r);
+
+  }
+}.
+
+
+
 module Sim1(V : RewMaliciousVerifier)  = {
-  module ZKP_HP = ZKP(HonestProver,V)
   proc sinit(p_a : hc_prob) : bool * (hc_com * hc_resp) = {
     var  g,bb,r;
     g <-  p_a;
     bb <$ {0,1};
     if (bb) {
-       r <@ ZKP_HP.run(p_a, witness, bb);
+       r <@ ZKP'.run(p_a, witness, bb);
     }else{
-       r <@ ZKP_HP.run(( compl_graph K), (compl_graph_cyc K), bb);
+       r <@ ZKP'.run(( compl_graph K), (compl_graph_cyc K), bb);
     }
     return (bb, r);
   }
 
   proc run(pa : hc_prob)   = {
-    var b',b,zryb,result,vstat, hpstat;
+    var b',b,zryb,result,vstat;
     vstat <@ V.getState();
-    hpstat <- (HonestProver.pi_w, HonestProver.pi_gwco, HonestProver.fal,
-    HonestProver.prm, HonestProver.w, HonestProver.g);
     (b',zryb) <@ sinit(pa);
     b <@ V.challenge(pa, zryb.`1);
     result <@ V.summitup(pa, zryb.`2);
     if (b <> b'){
       V.setState(vstat);
-      (HonestProver.pi_w, HonestProver.pi_gwco, HonestProver.fal,
-        HonestProver.prm, HonestProver.w, HonestProver.g) <- hpstat;
     }
     return (b = b', result);
   }
 }.
 
 section.
-declare module V <: RewMaliciousVerifier {-HonestProver}.
+declare module V <: RewMaliciousVerifier {-HonestProver, -ZKT.Hyb.Count, -ZKT.Hyb.HybOrcl}.
 
 
 declare axiom V_summitup_ll : islossless V.summitup.
@@ -85,10 +99,10 @@ declare axiom rewindable_V_plus :
 
 
 
-lemma sim1_rew_ph : forall (x : (glob V) * (glob Sim1)),
+lemma sim1_rew_ph : forall (x : (glob V) ),
     phoare[ Sim1(V).run :
-             ((glob V), (glob Sim1)) = x
-                 ==> ! res.`1 => ((glob V), (glob Sim1)) = x] = 1%r.
+             ((glob V)) = x
+                 ==> ! res.`1 => ((glob V)) = x] = 1%r.
 proof. progress.
 exists* (glob V). elim* => V_v.
 progress.
@@ -96,32 +110,36 @@ elim rewindable_V_plus.
 move => fA [s1 [s2 [s3]]] [s4 [ s5 [s6 s7]]].
 proc.
 seq 1 : (V_v = (glob V) /\ vstat = fA V_v /\
-  ((glob V),
-   (HonestProver.pi_w, HonestProver.pi_gwco, HonestProver.fal,
-    HonestProver.prm, HonestProver.w, HonestProver.g)) =
+  ((glob V)) =
   x).
 call (_: true ==> true). auto. skip. auto.
 call (s2 V_v).
 skip. progress.
 wp.
-seq 4 : (vstat = fA V_v /\ x = (V_v, hpstat)) 1%r.
+seq 3 : (vstat = fA V_v /\ x = (V_v)) 1%r.
 call (_:true).  call (_:true). call (_:true). auto. wp.  auto.
 simplify. call V_summitup_ll. call V_challenge_ll. sp.
 conseq (_: true ==> true). progress.  
 call (_:true). sp. 
 seq 1 : (true). rnd. skip. auto. rnd.  skip. smt.
-if. call (_:true). call P_response_ll.
-call P_commitment_ll. skip. auto. skip. auto.
-call (_:true). call P_response_ll.
-call P_commitment_ll. auto. auto. hoare. auto. auto. auto.
+if. call (_:true). wp. simplify. rnd.
+conseq (_: true ==> true). progress. 
+smt (djoinmap_weight Com_lossless).
+ wp.  rnd. skip. smt (perm_d_lossless).
+skip. auto.
+call (_:true).
+wp. simplify. rnd.
+conseq (_: true ==> true). progress. 
+smt (djoinmap_weight Com_lossless).
+ wp.  rnd. skip. smt (perm_d_lossless).
+ auto.  hoare. auto. auto. auto.
 case (b = b').
 rcondf 1. skip. auto. skip. auto.
 rcondt 1. skip. auto. wp. call (s5 V_v). skip. auto. 
-progress.  smt.
 hoare. simplify.
-call (_:true). call (_:true). call (_:true). auto.
-wp. 
-skip. auto. auto.  hoare. simplify. 
+call (_:true). call (_:true). conseq (_: _ ==> true). auto. 
+auto.
+auto.   hoare. simplify. 
 call (s3 V_v). skip. progress. auto.
 qed.
 
@@ -166,8 +184,8 @@ end section.
 module HP'= HonestProver.
 
 section.
-declare module V <: RewMaliciousVerifier {-HonestProver, -HP'}.
-declare module D <: ZKDistinguisher {-V,-HonestProver, -HP'}.
+declare module V <: RewMaliciousVerifier {-HonestProver, -HP', -ZKT.Hyb.Count, -ZKT.Hyb.HybOrcl}.
+declare module D <: ZKDistinguisher {-HonestProver, -HP'}.
 
 declare axiom V_summitup_ll : islossless V.summitup.
 
@@ -289,9 +307,11 @@ ZKDB ~ Sim1
 
 *)
 
+declare axiom jk : equiv [ D.guess ~ D.guess : ={arg, glob V, glob ZKT.Hyb.Count, glob ZKT.Hyb.HybOrcl} ==> ={res} ].
+
 local lemma sim_0_1 (g : hc_prob) (w: hc_wit):  K = size w => zk_relation g w =>
   equiv [ Sim1_0(V,D).simulate ~ Sim1_1(V).simulate : 
-               g = arg{2}.`1 /\ w = arg{2}.`2 /\ ={arg} /\ ={glob V, glob D} ==> ={res} ].
+               g = arg{2}.`1 /\ w = arg{2}.`2 /\ ={arg} /\ ={glob V, glob ZKT.Hyb.Count, glob ZKT.Hyb.HybOrcl} ==> ={res} ].
 proof. move => sas ishc. proc.
 inline Sim1_0(V,D).sinit.
 inline Sim1_1(V).sinit. 
@@ -302,18 +322,18 @@ seq 1 1 : (p_a{2} = pa{2} /\ (g,w) = (pa,wa){2} /\
   p_a{1} = pa{1} /\
   g{1} = p_a{1} /\
 
-  pa{1} = pa{2} /\ ={glob V, glob D,wa} /\ bb{1} = bb{2}).
+  pa{1} = pa{2} /\ ={glob V,wa, glob ZKT.Hyb.Count, glob ZKT.Hyb.HybOrcl} /\ bb{1} = bb{2}).
 rnd. skip. progress.  
 if. auto. 
-call (_:true).
+call jk.
 call (_:true).
 wp. inline*. wp.  call (_:true).
  wp.  rnd.  wp. rnd. wp. skip. progress.
 rewrite H. simplify. auto. 
-seq 1 1 : (={r,bb, glob V,glob D,pa,wa} /\ !bb{1}).
+seq 1 1 : (={r,bb, glob V,pa,wa, glob ZKT.Hyb.Count, glob ZKT.Hyb.HybOrcl} /\ !bb{1}).
 inline*. 
 seq  13 13 : (
-   !b1{1} /\ b1{1} = b1{2} /\ ={pa,c,wa, HP'.pi_w, HP'.pi_gwco,bb, glob V, glob D} /\ !bb{1} ).
+   !b1{1} /\ b1{1} = b1{2} /\ ={pa,c,wa, HP'.pi_w, HP'.pi_gwco,bb, glob V, glob ZKT.Hyb.Count, glob ZKT.Hyb.HybOrcl} /\ !bb{1} ).
 wp.  rnd. wp. 
 rnd  
  (fun (f : permutation) => compose f (inv (mk_perm HP'.w{2})))
@@ -353,7 +373,9 @@ rewrite map_comp.
 rewrite inv_prop3.
 elim ishc. progress. smt. smt.
 wp.   skip. progress. 
-rewrite H.  simplify. auto. sim.
+rewrite H.  simplify. auto. 
+call jk.
+call (_:true). call (_:true). wp.  skip. progress.
 qed.
 
 
@@ -450,7 +472,7 @@ local module Sim1_3(V : MaliciousVerifier) = {
 
 local lemma sim_2_3 (g : hc_prob)(w: hc_wit): zk_relation g w =>
   equiv [ Sim1_2(V).simulate ~ Sim1_3(V).simulate : 
-               arg{1}.`1 = g /\ arg{1}.`2 = w /\ ={arg} /\ ={glob V, glob D} ==> ={res} ].
+               arg{1}.`1 = g /\ arg{1}.`2 = w /\ ={arg} /\ ={glob V, glob ZKT.Hyb.Count, glob ZKT.Hyb.HybOrcl} ==> ={res} ].
 move => ishc.
 proc.
 inline Sim1_2(V).sinit.
@@ -464,10 +486,14 @@ seq 1 1 : (p_a{2} = pa{2} /\
   p_a{1} = pa{1} /\
   w_a{1} = wa{1} /\
   g{1} = p_a{1} /\
-   (pa{1}, wa{1}) = (pa{2}, wa{2}) /\ ={glob V, glob D} /\ bb{1} = bb{2}).
+   (pa{1}, wa{1}) = (pa{2}, wa{2}) /\ ={glob V, glob ZKT.Hyb.Count, glob ZKT.Hyb.HybOrcl} /\ bb{1} = bb{2}).
 rnd. skip. progress. 
 case (bb{1} = true).
-rcondt {1} 1. progress. sim.
+rcondt {1} 1. progress.  
+seq 4 4 : ((b{1} = b'{1}) = (b{2} = b'{2}) /\ ={pa,wa, result, glob V, glob ZKT.Hyb.Count, glob ZKT.Hyb.HybOrcl}). sim.
+call jk. skip. progress.
+
+
 rcondf {1} 1. progress. skip. smt.
 seq 1 1 : (p_a{2} = pa{2} /\
   w_a{2} = wa{2} /\
@@ -475,10 +501,10 @@ seq 1 1 : (p_a{2} = pa{2} /\
   p_a{1} = pa{1} /\
   w_a{1} = wa{1} /\
   g{1} = p_a{1} /\
- (pa{1}, wa{1}) = (pa{2}, wa{2}) /\ ={glob V, glob D} /\ bb{1} = bb{2} /\ r{1} = r{2}).
+ (pa{1}, wa{1}) = (pa{2}, wa{2}) /\ ={glob V, glob ZKT.Hyb.Count, glob ZKT.Hyb.HybOrcl} /\ bb{1} = bb{2} /\ r{1} = r{2}).
 symmetry.
 call (zkp_hp'_hp g w ). simplify. skip. progress.
-sim.
+call jk. call (_:true). call (_:true). wp. skip. progress.
 qed.
 
 
@@ -499,9 +525,12 @@ local module Sim1_4(V : MaliciousVerifier) = {
 
 local lemma sim_3_4:
   equiv [ Sim1_3(V).simulate ~ Sim1_4(V).simulate : 
-               arg{1} = arg{2} /\ ={glob V, glob D} ==> ={res} ].
-proc. sim. 
+               arg{1} = arg{2} /\ ={glob V, glob ZKT.Hyb.Count, glob ZKT.Hyb.HybOrcl} ==> ={res} ].
+proc. 
+seq 3 5 : (={glob V, glob ZKT.Hyb.Count, glob ZKT.Hyb.HybOrcl, pa,wa,result} /\ (b{1} = b'{1}) = (b{2} = bb{2})).
+sim.
 inline*. sp. wp. rnd. wp. rnd. wp.  rnd. skip. progress.
+call jk. skip. progress.
 qed.
 
 
@@ -522,8 +551,9 @@ local module Sim1_5(V : MaliciousVerifier) = {
 
 local lemma sim_4_5: 
   equiv [ Sim1_4(V).simulate ~ Sim1_5(V).simulate : 
-               arg{1} = arg{2} /\ ={glob V, glob D} ==> ={res} ].
-proc. sim. 
+               arg{1} = arg{2} /\ ={glob V, glob ZKT.Hyb.Count, glob ZKT.Hyb.HybOrcl} ==> ={res} ].
+proc. 
+call jk. 
 inline*. sp. wp. call (_:true). 
 call (_:true).  wp. rnd. wp. rnd.  wp. rnd. skip.
 progress.
@@ -547,8 +577,10 @@ local module Sim1_6(V : MaliciousVerifier) = {
 
 local lemma sim_5_6: 
   equiv [ Sim1_5(V).simulate ~ Sim1_6(V).simulate : 
-               arg{1} = arg{2} /\ ={glob V, glob D} ==> ={res} ].
-proc. swap {1} 5 -1. sim. swap {2} 3 -1. sim. qed.
+               arg{1} = arg{2} /\ ={glob V, glob ZKT.Hyb.Count, glob ZKT.Hyb.HybOrcl} ==> ={res} ].
+proc. swap {1} 5 -1. call jk.  swap {2} 3 -1. call (_:true). inline*. wp.  call (_:true). wp.
+rnd.  wp.  rnd. wp.  rnd. wp. skip. progress.
+qed.
 
 
 local module Sim1_7(V : MaliciousVerifier) = {
@@ -568,10 +600,10 @@ local module Sim1_7(V : MaliciousVerifier) = {
 
 local lemma sim_6_7: 
   equiv [ Sim1_6(V).simulate ~ Sim1_7(V).simulate : 
-               arg{1} = arg{2} /\ ={glob V, glob D, glob HonestProver} ==> 
+               arg{1} = arg{2} /\ ={glob V, glob HonestProver, glob ZKT.Hyb.Count, glob ZKT.Hyb.HybOrcl} ==> 
    res.`1{1} /\ res.`2{1} <=>  res.`1{2} /\ res.`2{2} ].
 proc. sp. 
-seq 3 3 : (={b,bb,r1,  wa, pa, glob V, glob D, glob HonestProver}).
+seq 3 3 : (={b,bb,r1,  wa, pa, glob V, glob HonestProver, glob ZKT.Hyb.Count, glob ZKT.Hyb.HybOrcl}).
 call (_:true). rnd. simplify.
 inline*. wp.  rnd. wp.  rnd. wp.  skip. progress.
 case (b{1} <> bb{1}).
@@ -582,7 +614,7 @@ call {2} (_:true ==> true). apply V_summitup_ll2.
 call {1} (_:true ==> true). proc. wp. skip. auto.
 call {2} (_:true ==> true). proc. wp. skip. auto.
 skip.  smt.
-sim. 
+call jk.  inline*. call (_:true). wp.  skip. progress.
 qed.
 
 
@@ -603,9 +635,11 @@ local module Sim1_8(V : MaliciousVerifier) = {
 
 local lemma sim_7_8: 
   equiv [ Sim1_7(V).simulate ~ Sim1_8(V).simulate : 
-               arg{1} = arg{2} /\ ={glob V, glob D} ==> ={res} ].
+               arg{1} = arg{2} /\ ={glob V,  glob ZKT.Hyb.Count, glob ZKT.Hyb.HybOrcl} ==> ={res} ].
 proc. swap {1} 3 4.
-seq 6 6 : (={rb}). sim. 
+seq 6 6 : (={rb}). call jk. call (_:true). inline*. wp. call (_:true). wp.  rnd. wp.
+rnd. wp. skip. progress.
+
 exists* b{1}. elim*. progress.
 rnd (fun b => b ^^ !b_L).
 skip. progress. smt. smt.
@@ -626,59 +660,61 @@ local module Sim1_9(V : MaliciousVerifier) = {
 
 local lemma sim_8_9: 
   equiv [ Sim1_8(V).simulate ~ Sim1_9(V).simulate : 
-               arg{1} = arg{2} /\ ={glob V, glob D, glob HonestProver} ==> ={res} ].
-proc. inline*. sim. progress. smt.
+               arg{1} = arg{2} /\ ={glob V, glob HonestProver,  glob ZKT.Hyb.Count, glob ZKT.Hyb.HybOrcl} ==> ={res} ].
+proc. inline*. rnd. wp. call jk. progress. call (_:true). wp.  call (_:true). wp.  rnd. wp. 
+rnd.  wp. skip. progress.
 qed.
 
 
 local lemma sim_2_9 g w: zk_relation g w =>
   equiv [ Sim1_2(V).simulate ~ Sim1_9(V).simulate : 
-              g = arg{1}.`1 /\ w = arg{1}.`2 /\ arg{1} = arg{2} /\ ={glob V, glob D, glob HonestProver} ==> 
+              g = arg{1}.`1 /\ w = arg{1}.`2 /\ arg{1} = arg{2} /\ ={glob V, glob HonestProver, glob ZKT.Hyb.Count, glob ZKT.Hyb.HybOrcl} ==> 
   res.`1{1} /\ res.`2{1} <=>  res.`1{2} /\ res.`2{2} ].
 move => ishc.
 transitivity Sim1_3(V).simulate 
-(g = arg{1}.`1 /\ w = arg{1}.`2 /\ arg{1} = arg{2} /\ ={glob V, glob D, glob HonestProver} ==> 
-  res.`1{1} /\ res.`2{1} <=>  res.`1{2} /\ res.`2{2}) (arg{1} = arg{2} /\ ={glob V, glob D, glob HonestProver} ==> 
+(g = arg{1}.`1 /\ w = arg{1}.`2 /\ arg{1} = arg{2} /\ ={glob V, glob ZKT.Hyb.Count, glob ZKT.Hyb.HybOrcl, glob HonestProver} ==> 
+  res.`1{1} /\ res.`2{1} <=>  res.`1{2} /\ res.`2{2}) (arg{1} = arg{2} /\ ={glob V,  glob HonestProver, glob ZKT.Hyb.Count, glob ZKT.Hyb.HybOrcl} ==> 
   res.`1{1} /\ res.`2{1} <=>  res.`1{2} /\ res.`2{2}). progress. smt. smt.
 conseq (sim_2_3 g w ishc). smt. auto. 
 transitivity Sim1_4(V).simulate 
-(arg{1} = arg{2} /\ ={glob V, glob D, glob HonestProver} ==> 
-  res.`1{1} /\ res.`2{1} <=>  res.`1{2} /\ res.`2{2}) (arg{1} = arg{2} /\ ={glob V, glob D, glob HonestProver} ==> 
+(arg{1} = arg{2} /\ ={glob V, glob HonestProver, glob ZKT.Hyb.Count, glob ZKT.Hyb.HybOrcl} ==> 
+  res.`1{1} /\ res.`2{1} <=>  res.`1{2} /\ res.`2{2}) (arg{1} = arg{2} /\ ={glob V,  glob HonestProver, glob ZKT.Hyb.Count, glob ZKT.Hyb.HybOrcl} ==> 
   res.`1{1} /\ res.`2{1} <=>  res.`1{2} /\ res.`2{2}). progress. smt. smt.
 conseq sim_3_4. auto. auto.
 transitivity Sim1_5(V).simulate 
-(arg{1} = arg{2} /\ ={glob V, glob D, glob HonestProver} ==> 
-  res.`1{1} /\ res.`2{1} <=>  res.`1{2} /\ res.`2{2}) (arg{1} = arg{2} /\ ={glob V, glob D, glob HonestProver} ==> 
+(arg{1} = arg{2} /\ ={glob V, glob HonestProver, glob ZKT.Hyb.Count, glob ZKT.Hyb.HybOrcl} ==> 
+  res.`1{1} /\ res.`2{1} <=>  res.`1{2} /\ res.`2{2}) (arg{1} = arg{2} /\ ={glob V, glob HonestProver, glob ZKT.Hyb.Count, glob ZKT.Hyb.HybOrcl} ==> 
   res.`1{1} /\ res.`2{1} <=>  res.`1{2} /\ res.`2{2}). progress. smt. smt.
 conseq sim_4_5. auto. auto.
 transitivity Sim1_6(V).simulate 
-(arg{1} = arg{2} /\ ={glob V, glob D, glob HonestProver} ==> 
-  res.`1{1} /\ res.`2{1} <=>  res.`1{2} /\ res.`2{2}) (arg{1} = arg{2} /\ ={glob V, glob D, glob HonestProver} ==> 
+(arg{1} = arg{2} /\ ={glob V,  glob HonestProver, glob ZKT.Hyb.Count, glob ZKT.Hyb.HybOrcl} ==> 
+  res.`1{1} /\ res.`2{1} <=>  res.`1{2} /\ res.`2{2}) (arg{1} = arg{2} /\ ={glob V, glob HonestProver, glob ZKT.Hyb.Count, glob ZKT.Hyb.HybOrcl} ==> 
   res.`1{1} /\ res.`2{1} <=>  res.`1{2} /\ res.`2{2}). progress. smt. smt.
 conseq sim_5_6. auto. auto.
 transitivity Sim1_7(V).simulate 
-(arg{1} = arg{2} /\ ={glob V, glob D, glob HonestProver} ==> 
-  res.`1{1} /\ res.`2{1} <=>  res.`1{2} /\ res.`2{2}) (arg{1} = arg{2} /\ ={glob V, glob D, glob HonestProver} ==> 
+(arg{1} = arg{2} /\ ={glob V, glob HonestProver, glob ZKT.Hyb.Count, glob ZKT.Hyb.HybOrcl} ==> 
+  res.`1{1} /\ res.`2{1} <=>  res.`1{2} /\ res.`2{2}) (arg{1} = arg{2} /\ ={glob V, glob HonestProver, glob ZKT.Hyb.Count, glob ZKT.Hyb.HybOrcl} ==> 
   res.`1{1} /\ res.`2{1} <=>  res.`1{2} /\ res.`2{2}). progress. smt. smt.
-conseq sim_6_7. auto. auto.
+conseq sim_6_7. auto. 
 transitivity Sim1_8(V).simulate 
-(arg{1} = arg{2} /\ ={glob V, glob D, glob HonestProver} ==> 
-  res.`1{1} /\ res.`2{1} <=>  res.`1{2} /\ res.`2{2}) (arg{1} = arg{2} /\ ={glob V, glob D, glob HonestProver} ==> 
+(arg{1} = arg{2} /\ ={glob V, glob HonestProver, glob ZKT.Hyb.Count, glob ZKT.Hyb.HybOrcl} ==> 
+  res.`1{1} /\ res.`2{1} <=>  res.`1{2} /\ res.`2{2}) (arg{1} = arg{2} /\ ={glob V, glob HonestProver, glob ZKT.Hyb.Count, glob ZKT.Hyb.HybOrcl} ==> 
   res.`1{1} /\ res.`2{1} <=>  res.`1{2} /\ res.`2{2}). progress. smt. smt.
 conseq sim_7_8. auto. auto.
-conseq sim_8_9. auto.
+conseq sim_8_9. auto. auto.
 qed.
 
 
 local lemma sim_9_10: 
   equiv [ Sim1_9(V).simulate ~ ZKD(HonestProver,V,D).main : 
-               arg{1} = arg{2} /\ ={glob V, glob D, glob HonestProver} 
+               arg{1} = arg{2} /\ ={glob V, glob HonestProver, glob ZKT.Hyb.Count, glob ZKT.Hyb.HybOrcl} 
                   ==> res.`2{1} = res{2} ].
 proc*.  
 inline Sim1_9(V).simulate.
 wp . rnd {1}.
-simplify. sp.  sim.
-(* inline*. sim. wp.  skip. progress. *)
+simplify. sp.  
+inline*. wp. call jk. call (_:true). wp. call (_:true). wp.  rnd. wp. rnd. wp.  skip.
+progress.
 qed.
 
 
@@ -693,8 +729,11 @@ qed.
 local lemma sim_9_pr2 &m pa wa: 
    Pr[ Sim1_9(V).simulate(pa,wa) @ &m : res.`2 /\ res.`1 ]
    = Pr[ Sim1_9(V).simulate(pa, wa) @ &m : res.`2 /\ !res.`1  ].
-proof. byequiv.
-proc. seq 1 1 : (={rb}). sim. rnd (fun x => !x). 
+proof. byequiv (_: ={glob V, glob ZKT.Hyb.Count, glob ZKT.Hyb.HybOrcl, arg} ==> _).
+proc. seq 1 1 : (={rb}). 
+inline*. wp. call jk. wp. call (_:true). wp. call (_:true). wp. rnd.
+wp. rnd. wp.  skip. progress. 
+rnd (fun x => !x). 
 skip. progress. auto. auto.
 qed.
 
@@ -724,18 +763,17 @@ proof. move => ishc.
 have ->: 
   Pr[ ZKD(HonestProver,V,D).main(pa,wa) @ &m : res ]
   = Pr[ Sim1_9(V).simulate(pa,wa) @ &m : res.`2 ]. 
- byequiv (_: arg{1} = arg{2} /\ ={glob V, glob D, glob HonestProver}  ==> _). 
+ byequiv (_: arg{1} = arg{2} /\ ={glob V, glob HonestProver, glob ZKT.Hyb.Count, glob ZKT.Hyb.HybOrcl}  ==> _). 
  symmetry. conseq sim_9_10. progress;auto. auto. auto. auto.
 have ->: 
    Pr[Sim1_0(V,D).simulate(pa,wa) @ &m : res.`1 /\ res.`2]
     = Pr[ Sim1_1(V).simulate(pa,wa) @ &m : res.`1 /\ res.`2 ].
-   byequiv. 
-conseq (sim_0_1 pa wa _ _ ). smt.  simplify. smt. auto. auto. auto.
+   byequiv (_: ={glob V, glob ZKT.Hyb.Count, glob ZKT.Hyb.HybOrcl} /\ arg{2} = (pa, wa) /\ arg{1} = (pa, wa) ==> _). 
+conseq (sim_0_1 pa wa _ _ ).   simplify. progress. smt. auto. auto. auto.
 have h: 
    Pr[Sim1_0(V,D).simulate(pa,wa) @ &m : res.`1]
     = Pr[ Sim1_1(V).simulate(pa,wa) @ &m : res.`1].
-   byequiv. conseq (sim_0_1 pa wa _ _). smt. smt. auto. auto. auto.
-
+   byequiv (_: ={glob V, glob ZKT.Hyb.Count, glob ZKT.Hyb.HybOrcl} /\ arg{2} = (pa, wa) /\ arg{1} = (pa, wa) ==> _). conseq (sim_0_1 pa wa _ _). smt. smt. auto. auto. auto.
 rewrite sim_9_pr3.
 apply (ler_trans (2%r * 
     `|Pr[Sim1_1(V).simulate(pa,wa) @ &m : res.`1 /\ res.`2] -
@@ -749,8 +787,9 @@ apply pr_e2. smt.
 apply sim1ass.
 have ->: Pr[Sim1_9(V).simulate(pa, wa) @ &m : res.`2 /\ res.`1] =
  Pr[Sim1_2(V).simulate(pa,wa) @ &m : res.`1 /\ res.`2].
+
 byequiv (_: (pa,wa) = arg{1} /\ arg{1} = arg{2} 
- /\ ={glob V, glob D, glob HonestProver} ==> _). 
+ /\ ={glob V, glob HonestProver, glob ZKT.Hyb.Count, glob ZKT.Hyb.HybOrcl} ==> _). 
 symmetry. conseq (sim_2_9 pa wa ishc). smt. smt. auto. auto.
 smt (sim_1_2).
 qed.    
@@ -758,157 +797,109 @@ qed.
 
 
                                       
-local module Sim1'(V : MaliciousVerifier)  = {
-  module ZKP_HP = ZKP(HonestProver,V)
-  module ZKP_HP' = ZKP(HP',V)
-  proc sinit(p_a : hc_prob) : bool * (hc_com * hc_resp) = {
-    var  g,bb,r;
-    g <- p_a;
-    bb <$ {0,1};
-    if (bb) {
-       r <@ ZKP_HP.run(p_a, witness, bb);
-    }else{
-       r <@ ZKP_HP'.run((compl_graph K), (compl_graph_cyc K), bb);
-    }
-    return (bb, r);
-  }
-
-  proc run(pa : hc_prob)   = {
-    var b',b,zryb,result;
-    (b',zryb) <@ sinit(pa);
-    b <@ V.challenge(pa, zryb.`1);
-    result <@ V.summitup(pa, zryb.`2);
-    return (b = b', result);
-  }
-}.
 
 
-
-
-
-local lemma qqq &m (p : hc_prob) (w : hc_wit) :
-
-   islossless D.guess =>
-   islossless V.summitup =>
-   zk_relation p w =>  
-    `|Pr[RD(Sim1'(V), D).run(p, w) @ &m : fst res.`2 /\ res.`1] /
-         Pr[Sim1'(V).run(p) @ &m : fst res] 
-              - Pr[ ZKD(HonestProver,V,D).main(p,w) @ &m : res ]| <= 2%r * negl + 20%r * negl2.
-progress.
-have ->: Pr[RD(Sim1'(V), D).run(p, w) @ &m : fst res.`2 /\ res.`1]
- = Pr[ Sim1_0(V,D).simulate(p,w) @ &m : res.`1 /\ res.`2 ].
-progress. byequiv;auto. proc.
-call (_:true). simplify. inline   Sim1'(V).run. sp. wp. call (_:true).
-call (_:true). simplify. call(_:true).
-sim. skip. progress. 
-have ->: Pr[Sim1'(V).run(p) @ &m : fst res] = 
- Pr[ Sim1_0(V,D).simulate(p,w) @ &m : res.`1 ].
-progress. byequiv (_: _ ==> res{1}.`1 = res{2}.`1);auto. proc.
-call {2} H. simplify.  sp. wp. call (_:true).
-call (_:true). simplify. call(_:true).
-sim. skip. progress.  smt.
-apply (sim1_main  &m  p w). assumption.
+lemma sim110 p ww &m :    islossless D.guess =>
+ Pr[Sim1(V).run(p) @ &m : res.`1] =
+  Pr[ Sim1_0(V,D).simulate(p,ww) @ &m : res.`1 ].
+move => dll.
+byequiv (_: (p,ww) = arg{2} /\ arg{1} = arg{2}.`1
+   /\ ={glob V} ==> res.`1{1} = res.`1{2}).
+proc.  simplify.
+seq 1 0 : ((p = pa{2} /\ ww = wa{2}) /\ ={pa, glob V}).
+elim rewindable_V_plus.
+move => fA [s1 [s2 [s3]]] [s4 [ s5 [s6 s7]]].
+exists*  (glob V){1}. elim*. progress.
+call {1} (s2 V_L). skip. progress.
+seq 3 3 : ((b{1} = b'{1}) = (b{2} = b'{2})). sim.
+inline*. wp. sp.
+seq 1 1 : (  p_a{2} = pa{2} /\
+  g{2} = p_a{2} /\
+  p_a{1} = pa{1} /\
+  g{1} = p_a{1} /\ (p = pa{2} /\ ww = wa{2}) /\ ={pa, glob V,bb}). rnd. skip. progress.
+if. progress. sp. wp. rnd.  wp. rnd. wp. skip. progress.
+wp. rnd. wp. rnd. wp. skip. progress.
+if {1}. 
+elim rewindable_V_plus.
+move => fA [s1 [s2 [s3]]] [s4 [ s5 [s6 s7]]].
+call {1} s7. call {2} dll. skip.  auto.
+call {2} dll. skip. auto. auto. smt.
 qed.
 
 
 
+lemma sim1_prop &m (p : hc_prob) (ww : hc_wit) :
+   islossless D.guess =>
+   islossless V.summitup =>
+   zk_relation p ww =>  
+    `|Pr[RD(Sim1(V), D).run(p, ww) @ &m : fst res.`2 /\ res.`1] /
+         Pr[Sim1(V).run(p) @ &m : fst res] 
+              - Pr[ ZKD(HonestProver,V,D).main(p,ww) @ &m : res ]| <= 2%r * negl + 20%r * negl2.
 
-local lemma sim11v_eq N : 0 <= N => equiv [ Sim1(V).run ~ Sim1'(V).run :  ={glob D, glob  V, glob HP', glob HonestProver} /\ ={arg}   
-   ==> ={res} ].
-progress. proc. simplify. sim. 
-inline Sim1(V).sinit.
-inline Sim1'(V).sinit.
-seq 1 0 : ((={glob D} /\
-   ={glob V} /\
-   ={HP'.pi_gwco, HP'.pi_w,
-       HP'.fal, HP'.prm, HP'.w, HP'.g} /\
-   ={HonestProver.pi_w, HonestProver.pi_gwco, HonestProver.fal,
-       HonestProver.prm, HonestProver.w, HonestProver.g}) /\
-  ={pa}).
+progress.
+have ->: Pr[RD(Sim1(V), D).run(p, ww) @ &m : fst res.`2 /\ res.`1]
+ = Pr[ Sim1_0(V,D).simulate(p,ww) @ &m : res.`1 /\ res.`2 ].
+progress. byequiv (_: (p,ww) = arg{1} /\ arg{1} = arg{2}
+ /\ ={glob V,  glob ZKT.Hyb.Count, glob ZKT.Hyb.HybOrcl} ==> _).  proc. simplify.
+seq 1 3 : (={glob ZKT.Hyb.Count, glob ZKT.Hyb.HybOrcl} /\ (p = a{1} ) /\
+  (a{1} = pa{2} /\ w{1} = wa{2}) /\ r.`2{1} = result{2} /\ (r{1}.`1  <=> b{2} = b'{2}) /\ (b{2} = b'{2} => ={glob V})  ).
+inline Sim1(V).run. wp. sp. simplify.
+seq 4 3 :   (={Hyb.Count.c, Hyb.HybOrcl.l, Hyb.HybOrcl.l0} /\
+  p = a{1} /\
+  (a{1} = pa{2} /\ w{1} = wa{2}) /\
+  ={result} /\
+  (b0{1} = b'{1} <=> b{2} = b'{2}) /\ (b{2} = b'{2} => ={glob V})).  call (_:true). call (_:true).
+seq 1 0 : (  pa{1} = a{1} /\
+  (p = a{1} /\ ww = w{1}) /\
+  (a{1} = pa{2} /\ w{1} = wa{2}) /\
+  ={glob V, Hyb.Count.c, Hyb.HybOrcl.l, Hyb.HybOrcl.l0}). 
 elim rewindable_V_plus.
-move => fA [s1 [s2 [s3]]] [s4 [ s5 [s6 s7]]]. 
-exists* (glob V){1}. elim*. progress.
+move => fA [s1 [s2 [s3]]] [s4 [ s5 [s6 s7]]].
+exists*  (glob V){1}. elim*. progress.
 call {1} (s2 V_L). skip. progress.
-sp. wp. 
-seq 1 1 : ( p_a{2} = pa{2} /\
+inline*. wp. sp.
+seq 1 1 :     (p_a{2} = pa{2} /\
   g{2} = p_a{2} /\
   p_a{1} = pa{1} /\
   g{1} = p_a{1} /\
-  (={glob D} /\
-   ={glob V} /\
-   ={HP'.pi_gwco,    HP'.pi_w,
-       HP'.fal, HP'.prm, HP'.w, HP'.g} /\
-   ={HonestProver.pi_w, HonestProver.pi_gwco, HonestProver.fal,
-       HonestProver.prm, HonestProver.w, HonestProver.g}) /\
-  ={pa,bb}).
-rnd. skip. progress. if.  
-progress.
-seq 4 4 : (={result,b',b}).
-sim.
-if{1}.
-wp.
-call {1} (_: true ==> true). 
+  pa{1} = a{1} /\
+  (p = a{1} /\ ww = w{1}) /\
+  (a{1} = pa{2} /\ w{1} = wa{2}) /\
+  ={glob V, Hyb.Count.c, Hyb.HybOrcl.l, Hyb.HybOrcl.l0,bb}). rnd.  skip. progress.
+if. progress. wp.  rnd.  wp. rnd. wp. skip. progress.
+wp. rnd. wp. rnd. wp. skip. progress.
+case (b0{1} = b'{1}).
+rcondf {1} 1. progress. skip. progress.
+rcondt {1} 1. progress. call {1} (_:true ==> true). 
 elim rewindable_V_plus.
-move => fA [s1 [s2 [s3]]] [s4 [ s5 [s6 s7]]].  apply s7.
-    skip. auto. skip. auto.
-seq 4 4 : (={result,b',b}).
-sim.
-(* call (zkp_hp'_hp ((N, compl_graph N),(compl_graph_cyc N))).  *)
-(* apply compl_graph_prop.  auto. skip. progress.- *)
-if{1}.
-wp.
-call {1} (_: true ==> true). 
-elim rewindable_V_plus.
-move => fA [s1 [s2 [s3]]] [s4 [ s5 [s6 s7]]].  apply s7.
-skip. auto. skip. auto.
+move => fA [s1 [s2 [s3]]] [s4 [ s5 [s6 s7]]].
+apply s7. skip. smt. 
+case (b{2} = b'{2}). 
+call jk. skip.  progress. 
+call {1} H. call {2} H. skip. smt. auto. auto.
+rewrite (sim110 p ww &m H).
+apply (sim1_main  &m  p ww). assumption.
 qed.
 
 
 
-lemma sim1_prop &m (p : hc_prob) (w : hc_wit) 
-  : 
-   zk_relation p w =>  
-    `|Pr[RD(Sim1(V), D).run(p, w) @ &m : fst res.`2 /\ res.`1] /
-         Pr[Sim1(V).run(p) @ &m : fst res] 
-              - Pr[ ZKD(HonestProver,V,D).main(p,w) @ &m : res ]| <= 2%r * negl + 20%r * negl2.
-proof.
-progress.
-have ->: Pr[Sim1(V).run(p) @ &m : res.`1] 
-  = Pr[Sim1'(V).run(p) @ &m : res.`1].
-byequiv (_: 
-  ={glob D, glob  V, glob HP', glob HonestProver} /\   ={arg} /\ arg{1} = (p)   ==> res.`1{1} = res.`1{2});auto. 
-conseq (sim11v_eq K _). auto. progress. smt. smt.
-have ->: Pr[RD(Sim1(V), D).run(p, w) @ &m : res.`2.`1 /\ res.`1]
-  = Pr[RD(Sim1'(V), D).run(p, w) @ &m : res.`2.`1 /\ res.`1].
-byequiv (_:  ={glob D, glob  V, glob HP', glob HonestProver} /\   ={arg} /\ arg{1} =(p,w)   ==> ={res});auto. 
-proc.
-call (_:true). 
-call (sim11v_eq K) . smt. skip. progress. apply qqq. 
-apply D_run_ll.
-apply V_summitup_ll2.
-auto.
-qed.
+
+
+
 
 
 lemma sim1assc &m stat : 
  inv 2%r - negl2 <= Pr[Sim1(V).run(stat) @ &m : res.`1].
 progress.
-have ->: Pr[Sim1(V).run(stat) @ &m : res.`1]
- = Pr[Sim1'(V).run(stat) @ &m : res.`1].
-byequiv (_: 
-  ={glob D, glob  V, glob HP', glob HonestProver} /\   ={arg} /\ arg{1} = (stat) ==> res.`1{1} = res.`1{2});auto. 
-conseq (sim11v_eq K _). auto. smt.  auto. smt. smt.
-have ->: Pr[Sim1'(V).run(stat) @ &m : res.`1] = 
+have ->: Pr[Sim1(V).run(stat) @ &m : res.`1] = 
  Pr[Sim1_0(V,D).simulate(stat, witness) @ &m : res.`1] .
-progress. byequiv (_: _ ==> res{1}.`1 = res{2}.`1);auto. proc.
-call {2} D_run_ll. simplify. inline   Sim1'(V).run. sp. wp. call (_:true).
-call (_:true). simplify. call(_:true).
-sim. skip. progress.  smt.
+rewrite (sim110 stat  witness &m).
+apply D_run_ll.
+ 
 have f : `|Pr[Sim1_0(V, D).simulate(stat,  witness) @ &m : res.`1] - 1%r / 2%r|
  <= negl2. 
-apply sim1ass. smt.
+apply sim1ass. auto.  smt.
 qed.
-
 
 end section.
 
