case_studies/HamiltonBlum/Blum_ZeroKnowledge.ec
@@ -5,6 +5,9 @@ require import Permutation Blum_Basics Blum_Sim1Property.
 (* import DJMM. *)
 import OSS.
 
+
+clone import ZKT.SequentialComposition.
+
 clone import Statistical with op epsilon <- 2%r * negl + 20%r * negl2,
                               op sigma <- (1%r/2%r - negl2).
 
@@ -17,7 +20,8 @@ clone import RewBasics as Rew with type sbits <- sbits.
 section.
 
 declare module V <: RewMaliciousVerifier{-HonestProver, -ZKT.Hyb.HybOrcl,-ZKT.Hyb.Count, -HP'}.
-declare module D <: ZKDistinguisher{-HonestProver, -V, -ZKT.Hyb.HybOrcl,-ZKT.Hyb.Count, -HP' }.
+declare module D <: ZKDistinguisher{-HonestProver,  -ZKT.Hyb.HybOrcl,-ZKT.Hyb.Count, -HP' }.
+
 
 
 declare axiom Sim1_run_ll : forall (V0 <: RewMaliciousVerifier), islossless V0.challenge => islossless V0.summitup => islossless Sim1(V0).run.
@@ -26,7 +30,8 @@ declare axiom V_challenge_ll : islossless V.challenge.
 declare axiom D_guess_ll : islossless D.guess.
 declare axiom P_response_ll : islossless HonestProver.response.
 declare axiom P_commitment_ll : islossless HonestProver.commitment.
-
+declare axiom simn_simulate_ll : forall (V0 <: RewMaliciousVerifier), islossless V0.challenge 
+  => islossless V0.summitup => islossless SimN(Sim1, V0).simulate.
 declare axiom D_guess_prop : equiv[ D.guess ~ D.guess : ={glob V, arg} ==> ={res} ].
 
 declare axiom rewindable_V_plus :
@@ -39,6 +44,7 @@ declare axiom rewindable_V_plus :
          islossless V.setState).
 
 
+      
 lemma hc_statistical_zk stat wit  &m:
         zk_relation stat wit => 
         let real_prob = Pr[ZKReal(HonestProver, V, D).run(stat, wit) @ &m : res] in
@@ -50,17 +56,77 @@ apply (statistical_zk HonestProver Sim1  V D _ _ _ _ _ _ _ _ _ _  stat wit &m _)
 apply D_guess_ll. 
 proc*. call D_guess_prop. skip.  auto.
 move => x.
-apply (sim1_rew_ph V _ _ _ _ _ x). apply V_summitup_ll. apply V_challenge_ll. apply P_response_ll. apply P_commitment_ll.
+conseq (sim1_rew_ph V _ _ _ _ _  x.`1).  auto. auto.
+apply V_summitup_ll. apply V_challenge_ll. apply P_response_ll. apply P_commitment_ll.
 apply (rewindable_A_plus V). apply rewindable_V_plus.
 progress.
-apply (sim1_prop V D  _ _  _ _ _  &m0 p w  _ );auto.  apply V_summitup_ll. apply (rewindable_A_plus V). apply rewindable_V_plus. 
+apply (sim1_prop V D  _ _  _ _ _  _ &m0 p w  _ );auto.  apply V_summitup_ll. apply (rewindable_A_plus V). apply rewindable_V_plus. 
 apply D_guess_ll. apply V_summitup_ll. apply V_challenge_ll. 
+conseq D_guess_prop. auto. apply D_guess_ll. apply V_summitup_ll.
 progress.
-apply (sim1assc V D _ _ _ _ _ &m0 stat0 ).  apply V_summitup_ll. apply (rewindable_A_plus V). apply rewindable_V_plus. apply D_guess_ll. apply V_summitup_ll.
+apply (sim1assc V D _ _ _ _ _ _ &m0 stat0 ).  apply V_summitup_ll. apply (rewindable_A_plus V). apply rewindable_V_plus. apply D_guess_ll. apply V_summitup_ll.
 apply V_challenge_ll. 
  progress. 
-
+conseq D_guess_prop. auto.
+auto.
 qed.
 
 
-end section.
+
+
+lemma hc_statistical_zk_iter stat wit &m:
+        zk_relation stat wit =>
+        let real_prob = Pr[ZKRealAmp(HonestProver, V, D).run(stat, wit) @ &m : res] in
+        let ideal_prob = Pr[ZKIdeal(SimAmp(SimN(Sim1)), V, D).run(stat, wit) @ &m : res] in
+          `|ideal_prob - real_prob| <= ZKT.n%r * ((2%r * negl + 20%r * negl2) + 2%r * (1%r- (1%r/2%r - negl2)) ^ OSS.N).
+progress.
+apply (zk_seq HonestProver (SimN(Sim1)) V D _ _ _ _ _ _ _ &m  ((2%r * negl + 20%r * negl2) + 2%r * (1%r- (1%r/2%r - negl2)) ^ OSS.N) stat wit). 
+progress.  
+apply (simn_simulate_ll V0). auto. auto.
+apply V_summitup_ll. apply V_challenge_ll. apply P_response_ll.
+apply P_commitment_ll. apply D_guess_ll.
+apply D_guess_prop.
+smt.
+progress.
+apply (statistical_zk HonestProver Sim1  V (Di(D, SimN(Sim1), V)) _ _ _ _ _ _ _ _ _ _  stat wit &n _).
+apply Sim1_run_ll.
+apply V_summitup_ll. apply V_challenge_ll. apply P_response_ll.
+apply P_commitment_ll. 
+proc. 
+call D_guess_ll. sp.
+while (true) (ZKT.n - ZKT.Hyb.HybOrcl.l). progress.
+wp. call (simn_simulate_ll V). apply V_challenge_ll. apply V_summitup_ll.  skip. smt.
+skip. smt.
+proc. 
+call D_guess_prop. sim.
+progress.
+proc*.  
+call (sim1_rew_ph V _ _ _ _ _ x.`1).  apply V_summitup_ll.
+apply V_challenge_ll. apply P_response_ll.
+apply P_commitment_ll. 
+apply (rewindable_A_plus V). apply rewindable_V_plus.  skip. auto. progress.
+rewrite (sim1_prop V (Di(D, SimN(Sim1), V))).
+apply V_summitup_ll.  apply (rewindable_A_plus V). apply rewindable_V_plus.
+proc. 
+call D_guess_ll. sp.
+while (true) (ZKT.n - ZKT.Hyb.HybOrcl.l). progress.
+wp. call (simn_simulate_ll V).  apply V_challenge_ll. apply V_summitup_ll. 
+skip. smt. skip. smt.
+apply V_summitup_ll. apply V_challenge_ll. 
+proc. call D_guess_prop. sim. 
+proc. call D_guess_ll. sp.
+while (true) (ZKT.n - ZKT.Hyb.HybOrcl.l). progress. wp. 
+call (simn_simulate_ll V).  apply V_challenge_ll. apply V_summitup_ll.  skip. smt.
+skip. smt. apply V_summitup_ll. auto.
+progress.
+rewrite (sim1assc V D _ _ _ _  _  _ &m0 stat0). 
+apply V_summitup_ll.
+apply (rewindable_A_plus V).
+apply rewindable_V_plus. 
+apply D_guess_ll. 
+apply V_summitup_ll.
+apply V_challenge_ll.
+conseq D_guess_prop.  auto. 
+auto. 
+qed.
+
